upd: some proof script of consistency1

coq/model/rBPFDecoder.v
@@ -288,10 +288,10 @@ Definition rbpf_decoder (pc : nat) (l : list u64) : option bpf_instruction :=
       let off : i16 := Word.repr (Int64.signed (decode_bpf data 16 16)) in
       let imm : i32 := Int.repr (Int64.signed (decode_bpf data 32 32)) in
       if Z.eqb (Byte.unsigned op) (Z.of_nat 0x18) then
-        if (length l <? pc + 1)
+        if (length l <? S pc)
           then None
         else
-          match nth_error l (pc + 1) with
+          match nth_error l (S pc) with
           | Some data2 =>
               let imm2 : i32 := Int.repr (Int64.signed (decode_bpf data2 32 32)) in
               match u4_to_bpf_ireg dst with
