coq/model/Consistency1.v
@@ -1,7 +1,8 @@
 From Coq Require Import ZArith List.
 From compcert.lib Require Import Integers Maps.
 From compcert.common Require Import Memory AST.
-From bpf.model Require Import ebpf rBPFCommType rBPFSyntax rBPFDecoder rBPFEncoder.
+From bpf.model Require Import ebpf rBPFCommType rBPFSyntax.
+From bpf.model Require Import rBPFDecoder rBPFEncoder BinSolver.
 
 Import ListNotations.
 
@@ -10,4 +11,23 @@ Lemma rbpf_encode_decode_consistency:
     (HL: list_in_list Int64.eq l_bin pc l = true)
     (Hencode: rbpf_encoder ins = l_bin),
       rbpf_decoder pc l = Some ins.
+Proof.
+  intros.
+  unfold rbpf_encoder, rbpf_decoder in *.
+  destruct ins; rewrite <- Hencode in HL; simpl in HL.
+  - destruct nth_error as [ins |] eqn: Hnth; [| inversion HL].
+    rewrite Bool.andb_true_iff in HL.
+    destruct HL as (Hins & HL).
+    destruct l as [| h0 l0]; [inversion HL |].
+    destruct nth_error as [ins0 |] eqn: Hnth0 in HL.
+    rewrite Bool.andb_true_iff in HL.
+    destruct HL as (Hins0 & _).
+    apply Int64.same_if_eq in Hins, Hins0.
+    subst.
+    assert (Heq: Byte.unsigned (Byte.repr (Int64.unsigned (decode_bpf (
+      binary_to_u64 (Byte.repr 24)
+      (bpf_ireg_to_u4 d) 0%nat (Word.repr 0) i) 0 8))) = Z.of_nat 24).
+    { unfold binary_to_u64.
+      atp_de decode_bpf encode_bpf.
+      ...
 Admitted.
